---
layout: post
title: Cosine Rule on a Sphere
date: 2012-01-02 14:43:00
description: How to use the cosine rule on a sphere
tags: mathematics
related_posts: true
thumbnail: assets/img/Law-of-haversines.png
---

As all (well, at least those that can remember) 15+ year olds know, to find the length of a side of a non-right angled triangle you can't use Pythagoras' theorem and instead require the so called 'Cosine Rule'.

Simply, the cosine rule is used to find (for example) the length of side $$c$$ in:

<div class="row mt-3">
    <div class="col-sm mt-3 mt-md-0">
        {% include figure.liquid loading="eager" path="assets/img/Triangle_with_notations_2.png" class="img-fluid rounded z-depth-1" zoomable=true %}
    </div>
</div>

You use the following formula:

$$
c^2 = a^2 + b^2 - 2ab\cos(\gamma).
$$

But what happens if we move away from Euclidean Geometry and that our triangle is now sitting on a sphere? I.e.

<div class="row mt-3">
    <div class="col-sm mt-3 mt-md-0">
        {% include figure.liquid loading="eager" path="assets/img/Law-of-haversines.png" class="img-fluid rounded z-depth-1" zoomable=true %}
    </div>
</div>

Logic tells us that of course the same cosine rule can not be applied to find the side $$c$$. Instead we use an alternative formula, namely:

$$
\cos(c)=\cos(a)\cos(b)+\sin(a)\sin(b)\cos(C).
$$

The proof is relatively straight forward, try having a go before looking below:

Let $$\textbf{u}$$, $$\textbf{v}$$ and $$\textbf{w}$$ be unit vectors from the middle of the sphere to the points $$u$$, $$v$$ and $$w$$ of our triangle. The lengths of the sides are then give by the dot product:

$$
\begin{eqnarray*}
\cos(a) &=& \textbf{u}\cdot\textbf{v},\\
\cos(b) &=& \textbf{u}\cdot\textbf{w},\\
\cos(c) &=& \textbf{v}\cdot\textbf{w}.
\end{eqnarray*}
$$

The angle $$C$$ is the inverse cosine of two tangents, say $$\textbf{t}_a$$ and $$\textbf{t}_b$$, which are along the sides $$a$$ and $$b$$, i.e.

$$
\begin{eqnarray*}
C &=& \cos^{-1}(\textbf{t}_a\cdot\textbf{t}_b),\\
\cos(C) &=& \textbf{t}_a\cdot\textbf{t}_b.
\end{eqnarray*}
$$

But we know more information about these tangent vectors. For instance we know that the they are perpendicular to $$\textbf{u}$$ which is given by the component of $$\textbf{v}$$ perpendiculat to $$\textbf{u}$$.

This gives (once normalized):

$$
\textbf{t}_a=\frac{\textbf{v}-\textbf{u}(\textbf{u}\cdot\textbf{v})}{|\textbf{v}-\textbf{u}(\textbf{u}\cdot\textbf{v})|} = \frac{\textbf{v}-\textbf{u}\cos(a)}{\sin(a)}.
$$

Similarly,

$$
\textbf{t}_b=\frac{\textbf{w}-\textbf{u}(\textbf{u}\cdot\textbf{w})}{|\textbf{w}-\textbf{u}(\textbf{u}\cdot\textbf{w})|} = \frac{\textbf{w}-\textbf{u}\cos(b)}{\sin(b)}.
$$

So substituting these values into the above equation we get:

$$
\begin{eqnarray*}
\cos(C) &=& \frac{\textbf{v}-\textbf{u}\cos(a)}{\sin(a)}\cdotÂ \frac{\textbf{w}-\textbf{u}\cos(b)}{\sin(b)},\\
\cos(C) &=& \frac{\textbf{v}\cdot\textbf{w}-(\textbf{v}\cdot\textbf{u})\cos(b)-(\textbf{u}\cdot\textbf{w})\cos(a)+(\textbf{u}\cdot\textbf{u})\cos(a)\cos(b)}{\sin(a)\sin(b)},\\
\cos(C) &=& \frac{\cos(c)-\cos(a)\cos(b)}{\sin(a)\sin(b)}.
\end{eqnarray*}
$$

Which when rearranged gives the required cosine rule:

$$
\cos(c)=\cos(a)\cos(b)+\sin(a)\sin(b)\cos(C).
$$

Follow this link if you want to see the [sine rule on a sphere](https://seanelvidge.github.io/blog/2012/sine-rule-on-a-sphere/).
